keccak: attempt of verification with explicit array values using large records

Garden/Plonky3/keccak/round_flags.v
@@ -37,8 +37,177 @@ Definition eval_round_flags (is_first_row is_transition : bool) (local next : Ke
     assert_zeros (N := NUM_ROUNDS) (| Array.from_fn (| fun i => [[
       M.sub (|
         Array.get (| local.(KeccakCols.step_flags), i |),
-        Array.get (| next.(KeccakCols.step_flags), M.mod_ (| i + 1, NUM_ROUNDS |) |)
+        Array.get (| next.(KeccakCols.step_flags), (i + 1) mod NUM_ROUNDS |)
       |)
     ]] |) |)
   ]] in
   M.Pure tt.
+
+Definition eval_round_flags_step_flags
+    (is_first_row is_transition : bool)
+    (local next : Array.t Z NUM_ROUNDS) :
+    M.t unit :=
+  let* _ := when is_first_row [[
+    assert_one (| Array.get (| local, 0 |) |)
+  ]] in
+  let* _ := when is_first_row [[
+    assert_zeros (| Array.slice_from local 1 |)
+  ]] in
+  let* _ := when is_transition [[
+    assert_zeros (N := NUM_ROUNDS) (| Array.from_fn (| fun i => [[
+      M.sub (|
+        Array.get (| local, i |),
+        Array.get (| next, (i + 1) mod NUM_ROUNDS |)
+      |)
+    ]] |) |)
+  ]] in
+  M.Pure tt.
+
+(* Definition eval_round_flags_explicit
+    (is_first_row is_transition : bool)
+    (local next : KeccakColsExplicit.t) :
+    M.t unit :=
+  let* _ := when is_first_row [[
+    assert_one (| ExplicitArray.get local.(KeccakColsExplicit.step_flags) 0 |)
+  ]] in
+  let* _ := when is_first_row [[
+    assert_zeros (| ExplicitArray.slice_from local.(KeccakColsExplicit.step_flags) 1 |)
+  ]] in
+  (* let* _ := when is_transition [[
+    assert_zeros (N := NUM_ROUNDS) (| ExplicitArray.from_fn (| fun i => [[
+      M.sub (|
+        ExplicitArray.get local.(KeccakColsExplicit.step_flags) i,
+        ExplicitArray.get next.(KeccakColsExplicit.step_flags) ((i + 1) mod NUM_ROUNDS)
+      |)
+    ]] |) |)
+  ]] in *)
+  M.Pure tt. *)
+
+Module Spec.
+  Lemma spec_first_row (p : Z)
+      (local next : StepFlagsInput.t)
+      (H_p : IsPrime p) :
+    {{ M.eval p (eval_round_flags_step_flags true false
+        (StepFlagsInput.to_value local) (StepFlagsInput.to_value next)) 🔽
+      tt,
+      StepFlagsInput.to_value local = StepFlagsOutput.to_value 0
+    }}.
+  Proof.
+    destruct local.
+    cbn; unfold Pos.to_nat; cbn.
+    eapply Run.Equiv. {
+      progress repeat (
+        apply Run.Pure ||
+        eapply Run.Let ||
+        apply Run.Equal
+      ).
+    }
+    unfold StepFlagsInput.to_value, StepFlagsOutput.to_value, Array.from_fn_pure; cbn.
+    unfold Pos.to_nat; cbn.
+    split; sauto lq: on rew: off.
+  Qed.
+
+  Lemma spec_transition (p : Z)
+      (local : StepFlagsOutput.t)
+      (next : StepFlagsInput.t)
+      (H_p : IsPrime p) :
+    {{ M.eval p (eval_round_flags_step_flags false true
+        (StepFlagsOutput.to_value local) (StepFlagsInput.to_value next)) 🔽
+      tt,
+      StepFlagsInput.to_value next = StepFlagsOutput.to_value (local + 1)
+    }}.
+  Proof.
+    (* destruct next. *)
+    (* unfold StepFlagsOutput.to_value, Array.from_fn_pure; cbn.
+    unfold Pos.to_nat, Array.get; cbn. *)
+    eapply Run.Equiv; cbn. {
+      progress repeat (
+        apply Run.Pure ||
+        eapply Run.Let ||
+        apply Run.Equal
+      ).
+    }
+    replace local with 15 by admit.
+    cbn.
+    withcbn.
+    split; sauto lq: on rew: off.
+
+  Definition initial_step_flags : Array.t Z NUM_ROUNDS :=
+    Array.from_fn_pure (fun i =>
+      if i =? 0 then 1 else 0
+    ).
+
+  Definition initial_step_flags_explicit : ExplicitArray.t Z NUM_ROUNDS :=
+    ExplicitArray.from_fn (length := NUM_ROUNDS) (fun i =>
+      if i =? 0 then 1 else 0
+    ).
+
+  Definition shift (local_step_flags next_step_flags : Array.t Z NUM_ROUNDS) : Prop :=
+    forall i,
+      Array.get local_step_flags i =
+      Array.get next_step_flags ((i + 1) mod NUM_ROUNDS).
+
+  Definition spec (is_first_row is_transition : bool) (local next : KeccakCols.t) : Prop :=
+    if is_first_row then
+      local.(KeccakCols.step_flags) = initial_step_flags
+    else if is_transition then
+      shift local.(KeccakCols.step_flags) next.(KeccakCols.step_flags)
+    else
+      True.
+
+  Definition spec_step_flags (is_first_row is_transition : bool) (local next : Array.t Z NUM_ROUNDS) : Prop :=
+    if is_first_row then
+      local = initial_step_flags
+    else if is_transition then
+      shift local next
+    else
+      True.
+
+  Definition spec_step_flags_explicit (is_first_row is_transition : bool) (local next : ExplicitArray.t Z NUM_ROUNDS) : Prop :=
+    if is_first_row then
+      local = initial_step_flags_explicit
+    else if is_transition then
+      shift (ExplicitArray.to_array local) (ExplicitArray.to_array next)
+    else
+      True.
+
+  (* Notation "array [< >]" := (array.(Pair.x)) (at level 100).
+  Notation "array [< .. >]" := (array.(Pair.xs)) (at level 100). *)
+
+  Lemma spec_correct_step_flags (p : Z)
+    (local next : ExplicitArray.t Z NUM_ROUNDS)
+    (H_p : IsPrime p) :
+    let local_array := ExplicitArray.to_array local in
+    let next_array := ExplicitArray.to_array next in
+    {{ M.eval p (eval_round_flags_step_flags true false local_array next_array) 🔽
+      tt, spec_step_flags_explicit true false local next
+    }}.
+  Proof.
+    do 24 destruct local as [? local].
+    cbn; unfold Pos.to_nat; cbn.
+    eapply Run.Equiv. {
+      progress repeat (
+        apply Run.Pure ||
+        eapply Run.Let ||
+        apply Run.Equal
+      ).
+    }
+    split; sauto lq: on rew: off.
+  Qed.
+
+  Lemma spec_correct (p : Z) (is_first_row is_transition : bool) (local next : KeccakCols.t)
+    (H_p : IsPrime p)
+    (H_local : KeccakCols.Valid.t local)
+    (H_next : KeccakCols.Valid.t next) :
+    {{ M.eval p (eval_round_flags is_first_row is_transition local next) 🔽
+      tt, spec is_first_row is_transition local next
+    }}.
+  Proof.
+    destruct H_local, H_next.
+    (* Print Array.Valid.t.
+    destruct is_first_row, is_transition; cbn.
+    { eapply Run.Equiv. {
+        destruct local.(KeccakCols.step_flags).(Array.value).
+      }
+
+    } *)
